proof: show what action happened on the storage according to the logs

examples/ink_contracts/erc20.rs
@@ -57,6 +57,11 @@ struct Approval {
     value: Balance,
 }
 
+enum Event {
+    Transfer(Transfer),
+    Approval(Approval),
+}
+
 /// The ERC-20 error types.
 enum Error {
     /// Returned if not enough balance to fulfill a request is available.
@@ -73,7 +78,7 @@ impl Env {
         self.caller
     }
 
-    fn emit_event<Event>(&self, _event: Event) {
+    fn emit_event(&self, _event: Event) {
         unimplemented!()
     }
 }
@@ -95,11 +100,11 @@ impl Erc20 {
         let mut balances = Mapping::default();
         let caller = Self::init_env().caller();
         balances.insert(caller, total_supply);
-        Self::init_env().emit_event(Transfer {
+        Self::init_env().emit_event(Event::Transfer(Transfer {
             from: None,
             to: Some(caller),
             value: total_supply,
-        });
+        }));
         Self {
             total_supply,
             balances,
@@ -172,11 +177,11 @@ impl Erc20 {
         self.balances.insert(*from, from_balance - value);
         let to_balance = self.balance_of_impl(to);
         self.balances.insert(*to, to_balance + value);
-        self.env().emit_event(Transfer {
+        self.env().emit_event(Event::Transfer(Transfer {
             from: Some(*from),
             to: Some(*to),
             value,
-        });
+        }));
         Ok(())
     }
 
@@ -205,11 +210,11 @@ impl Erc20 {
     fn approve(&mut self, spender: AccountId, value: Balance) -> Result<()> {
         let owner = self.env().caller();
         self.allowances.insert((owner, spender), value);
-        self.env().emit_event(Approval {
+        self.env().emit_event(Event::Approval(Approval {
             owner,
             spender,
             value,
-        });
+        }));
         Ok(())
     }
 
