CoqOfRust/examples/default/examples/ink_contracts/Proofs/erc20.v
@@ -12,16 +12,19 @@ Import Simulations.M.Notations.
 Module State.
   Record t : Set := {
     storage : option erc20.Erc20.t;
+    events : list erc20.Event.t;
   }.
 
   Definition of_storage (storage : erc20.Erc20.t) : t := {|
     storage := Some storage;
+    events := [];
   |}.
 End State.
 
 Module Address.
   Inductive t : Set :=
   | storage : t
+  | events : t
   .
 End Address.
 
@@ -30,15 +33,19 @@ Module StateInstance.
     State.get_Set address :=
       match address with
       | Address.storage => erc20.Erc20.t
+      | Address.events => list erc20.Event.t
       end;
     State.read address state :=
       match address with
       | Address.storage => state.(State.storage)
+      | Address.events => Some state.(State.events)
       end;
     State.alloc_write address state value :=
       match address, value with
       | Address.storage, storage =>
         Some (state <| State.storage := Some storage |>)
+      | Address.events, events =>
+        Some (state <| State.events := events |>)
       end;
   }.
 
@@ -47,6 +54,14 @@ Module StateInstance.
     sauto lq: on rew: off.
   Qed.
 End StateInstance.
+
+Module Environment.
+  Definition t : Set :=
+    erc20.Env.t * M.Val (list erc20.Event.t).
+
+  Definition of_env (env : erc20.Env.t) : t :=
+    (env, Ref.mut_ref Address.events).
+End Environment.
 
 Definition sum_of_money (storage : erc20.Erc20.t) : Z :=
   Lib.Mapping.sum
@@ -81,12 +96,44 @@ Module Erc20.
   End Valid.
 End Erc20.
 
-Lemma account_id_eq_neq (x y : erc20.AccountId.t) :
-  x = y \/ x <> y.
-Proof.
-  destruct x as [[x]], y as [[y]].
-  destruct (Z.eq_dec x y); sfirstorder.
-Qed.
+Module AccountId.
+  Definition eqb (x y : erc20.AccountId.t) : bool :=
+    x.(erc20.AccountId.x0) ==u128 y.(erc20.AccountId.x0).
+
+  Lemma eqb_true (x y : erc20.AccountId.t) :
+    eqb x y = true ->
+    x = y.
+  Proof.
+    destruct x as [[x]], y as [[y]].
+    unfold
+      eqb,
+      BinOp.Pure.eq,
+      BinOp.Pure.make_comparison.
+    cbn; intros.
+    now replace x with y by lia.
+  Qed.
+
+  Lemma eqb_false (x y : erc20.AccountId.t) :
+    eqb x y = false ->
+    x <> y.
+  Proof.
+    destruct x as [[x]], y as [[y]].
+    unfold
+      eqb,
+      BinOp.Pure.eq,
+      BinOp.Pure.make_comparison.
+    cbn; intros.
+    intro; assert (x = y) by congruence.
+    lia.
+  Qed.
+
+  Lemma eq_or_neq (x y : erc20.AccountId.t) :
+    x = y \/ x <> y.
+  Proof.
+    destruct x as [[x]], y as [[y]].
+    destruct (Z.eq_dec x y); sfirstorder.
+  Qed.
+End AccountId.
 
 Module Mapping.
   Lemma insert_balances_is_valid from (diff : u128.t) storage
@@ -100,7 +147,7 @@ Module Mapping.
   Proof.
     constructor; try apply H_storage.
     eapply Lib.Mapping.Forall_insert;
-      sauto lq: on use: account_id_eq_neq.
+      sauto lq: on use: AccountId.eq_or_neq.
   Qed.
 
   Lemma insert_allowances_is_valid couple (diff : u128.t) storage
@@ -116,8 +163,8 @@ Module Mapping.
     constructor; cbn; try apply H_storage.
     eapply Lib.Mapping.Forall_insert; try assumption; try apply H_storage.
     intros [a1 a2] [b1 b2].
-    destruct (account_id_eq_neq a1 b1);
-      destruct (account_id_eq_neq a2 b2);
+    destruct (AccountId.eq_or_neq a1 b1);
+      destruct (AccountId.eq_or_neq a2 b2);
       hauto lq: on.
   Qed.
 End Mapping.
@@ -128,7 +175,7 @@ Module Env.
   (** The simulation [caller] is equal. *)
   Lemma run_caller (env : erc20.Env.t) (state : State.t) (logs : M.Logs) :
     let ref_env := Ref.Imm env in
-    {{ env, state, logs |
+    {{ Environment.of_env env, state, logs |
       erc20.Impl_erc20_Env_t.caller ref_env ⇓
       inl (Simulations.erc20.Env.caller env)
     | state, logs }}.
@@ -139,16 +186,20 @@ Module Env.
 
   (** The simulation [emit_event] is equal. *)
   Lemma run_emit_event
-    {E : Set}
     (env : erc20.Env.t)
-    (event : E)
+    (event : erc20.Event.t)
     (state : State.t)
     (logs : M.Logs) :
     let ref_env := Ref.Imm env in
-    {{ env, state, logs |
+    {{ Environment.of_env env, state, logs |
       erc20.Impl_erc20_Env_t.emit_event ref_env event ⇓
-      inl Simulations.erc20.Env.emit_event
-    | state, existS E event :: logs }}.
+      inl tt
+    | state <|
+        State.events :=
+          Simulations.erc20.Env.emit_event state.(State.events) event
+      |>,
+      logs
+    }}.
   Proof.
     run_symbolic.
   Qed.
@@ -159,7 +210,7 @@ End Env.
 Lemma run_env (env : erc20.Env.t) (storage : erc20.Erc20.t) (logs : M.Logs) :
   let state := State.of_storage storage in
   let self := Ref.mut_ref Address.storage in
-  {{ env, state, logs |
+  {{ Environment.of_env env, state, logs |
     erc20.Impl_erc20_Erc20_t.env self ⇓
     inl (Simulations.erc20.env env)
   | state, logs }}.
@@ -179,7 +230,7 @@ Lemma run_total_supply
     (logs : M.Logs) :
   let state := State.of_storage storage in
   let self := Ref.mut_ref Address.storage in
-  {{ env, state, logs |
+  {{ Environment.of_env env, state, logs |
     erc20.Impl_erc20_Erc20_t_2.total_supply self ⇓
     inl (Simulations.erc20.total_supply storage)
   | state, logs }}.
@@ -198,7 +249,7 @@ Lemma run_balance_of_impl
   let state := State.of_storage storage in
   let self := Ref.mut_ref Address.storage in
   let ref_owner : ref erc20.AccountId.t := Ref.Imm owner in
-  {{ env, state, logs |
+  {{ Environment.of_env env, state, logs |
     erc20.Impl_erc20_Erc20_t_2.balance_of_impl self ref_owner ⇓
     inl (Simulations.erc20.balance_of_impl storage owner)
   | state, logs }}.
@@ -235,7 +286,7 @@ Lemma run_balance_of
     (owner : erc20.AccountId.t) :
   let state := State.of_storage storage in
   let self := Ref.mut_ref Address.storage in
-  {{ env, state, logs |
+  {{ Environment.of_env env, state, logs |
     erc20.Impl_erc20_Erc20_t_2.balance_of self owner ⇓
     inl (Simulations.erc20.balance_of storage owner)
   | state, logs }}.
@@ -262,7 +313,7 @@ Lemma run_allowance_impl
   let self := Ref.mut_ref Address.storage in
   let ref_owner : ref erc20.AccountId.t := Ref.Imm owner in
   let ref_spender : ref erc20.AccountId.t := Ref.Imm spender in
-  {{ env, state, logs |
+  {{ Environment.of_env env, state, logs |
     erc20.Impl_erc20_Erc20_t_2.allowance_impl self ref_owner ref_spender ⇓
     inl (Simulations.erc20.allowance_impl storage owner spender)
   | state, logs }}.
@@ -300,7 +351,7 @@ Lemma run_allowance
     (spender : erc20.AccountId.t) :
   let state := State.of_storage storage in
   let self := Ref.mut_ref Address.storage in
-  {{ env, state, logs |
+  {{ Environment.of_env env, state, logs |
     erc20.Impl_erc20_Erc20_t_2.allowance self owner spender ⇓
     inl (Simulations.erc20.allowance storage owner spender)
   | state, logs }}.
@@ -342,17 +393,15 @@ Module Output.
   Record t {A : Set} : Set := {
     result : A + M.Exception;
     state : State.t;
-    logs : M.Logs;
   }.
   Arguments t : clear implicits.
 End Output.
 
 Definition lift_simulation {A : Set}
-  (simulation : MS? (erc20.Erc20.t * M.Logs) A)
-  (storage : erc20.Erc20.t)
-  (logs : M.Logs) :
+  (simulation : MS? Simulations.erc20.State.t A)
+  (storage : erc20.Erc20.t) :
   Output.t A :=
-  let '(result, (storage, logs)) := simulation (storage, logs) in
+  let '(result, (storage, events)) := simulation (storage, []) in
   let result :=
     match result with
     | inl result => inl result
@@ -360,8 +409,10 @@ Definition lift_simulation {A : Set}
     end in
   {|
     Output.result := result;
-    Output.state := State.of_storage storage;
-    Output.logs := logs;
+    Output.state := {|
+      State.storage := Some storage;
+      State.events := events;
+    |};
   |}.
 
 (** The simulation [transfer_from_to] is equal. *)
@@ -380,11 +431,11 @@ Lemma run_transfer_from_to
   let ref_to : ref erc20.AccountId.t := Ref.Imm to in
   let simulation :=
     lift_simulation
-      (Simulations.erc20.transfer_from_to from to value) storage logs in
-  {{ env, state, logs |
+      (Simulations.erc20.transfer_from_to from to value) storage in
+  {{ Environment.of_env env, state, logs |
     erc20.Impl_erc20_Erc20_t_2.transfer_from_to self ref_from ref_to value ⇓
     simulation.(Output.result)
-  | simulation.(Output.state), simulation.(Output.logs) }}.
+  | simulation.(Output.state), logs }}.
 Proof.
   unfold
     erc20.Impl_erc20_Erc20_t_2.transfer_from_to,
@@ -444,11 +495,11 @@ Lemma run_transfer
   let self := Ref.mut_ref Address.storage in
   let simulation :=
     lift_simulation
-      (Simulations.erc20.transfer env to value) storage logs in
-  {{ env, state, logs |
+      (Simulations.erc20.transfer env to value) storage in
+  {{ Environment.of_env env, state, logs |
     erc20.Impl_erc20_Erc20_t_2.transfer self to value ⇓
     simulation.(Output.result)
-  | simulation.(Output.state), simulation.(Output.logs) }}.
+  | simulation.(Output.state), logs }}.
 Proof.
   unfold erc20.Impl_erc20_Erc20_t_2.transfer,
     Simulations.erc20.transfer,
@@ -483,11 +534,11 @@ Lemma run_approve
   let self := Ref.mut_ref Address.storage in
   let simulation :=
     lift_simulation
-      (Simulations.erc20.approve env spender value) storage logs in
-  {{ env, state, logs |
+      (Simulations.erc20.approve env spender value) storage in
+  {{ Environment.of_env env, state, logs |
     erc20.Impl_erc20_Erc20_t_2.approve self spender value ⇓
     simulation.(Output.result)
-  | simulation.(Output.state), simulation.(Output.logs) }}.
+  | simulation.(Output.state), logs }}.
 Proof.
   unfold erc20.Impl_erc20_Erc20_t_2.approve,
     Simulations.erc20.approve.
@@ -513,11 +564,11 @@ Lemma run_transfer_from
   let self := Ref.mut_ref Address.storage in
   let simulation :=
     lift_simulation
-      (Simulations.erc20.transfer_from env from to value) storage logs in
-  {{ env, state, logs |
+      (Simulations.erc20.transfer_from env from to value) storage in
+  {{ Environment.of_env env, state, logs |
     erc20.Impl_erc20_Erc20_t_2.transfer_from self from to value ⇓
     simulation.(Output.result)
-  | simulation.(Output.state), simulation.(Output.logs) }}.
+  | simulation.(Output.state), logs }}.
 Proof.
   unfold erc20.Impl_erc20_Erc20_t_2.transfer_from,
     Simulations.erc20.transfer_from,
@@ -582,7 +633,7 @@ Lemma balance_of_impl_read_id
   let self : ref erc20.Erc20.t := Ref.mut_ref Address.storage in
   (* The value [owner] is an immediate value *)
   let ref_owner : ref erc20.AccountId.t := Ref.Imm owner in
-  {{ env, state, logs |
+  {{ Environment.of_env env, state, logs |
     erc20.Impl_erc20_Erc20_t_2.balance_of_impl self ref_owner ⇓
     (* expected output *)
     inl balance
@@ -652,7 +703,7 @@ Module ReadMessage.
       (message : t A) :
     let state := State.of_storage storage in
     let simulation := simulation_dispatch env storage message in
-    {{ env, state, logs |
+    {{ Environment.of_env env, state, logs |
       dispatch message ⇓
       inl simulation
     | state, logs }}.
@@ -715,7 +766,7 @@ Module WriteMessage.
   Definition simulation_dispatch
       (env : erc20.Env.t)
       (message : t) :
-      MS? (erc20.Erc20.t * M.Logs) ltac:(erc20.Result unit) :=
+      MS? Simulations.erc20.State.t ltac:(erc20.Result unit) :=
     match message with
     | transfer to value =>
       Simulations.erc20.transfer env to value
@@ -735,12 +786,12 @@ Module WriteMessage.
       (H_message : Valid.t message) :
     let simulation :=
       lift_simulation
-        (simulation_dispatch env message) storage logs in
+        (simulation_dispatch env message) storage in
     let state := State.of_storage storage in
-    {{ env, state, logs |
+    {{ Environment.of_env env, state, logs |
       dispatch message ⇓
       simulation.(Output.result)
-    | simulation.(Output.state), simulation.(Output.logs) }}.
+    | simulation.(Output.state), logs }}.
   Proof.
     destruct message; simpl.
     { apply run_transfer; scongruence. }
@@ -757,7 +808,7 @@ Lemma read_message_no_panic
     (logs : M.Logs) :
   let state := State.of_storage storage in
   exists result,
-  {{ env, state, logs |
+  {{ Environment.of_env env, state, logs |
     ReadMessage.dispatch message ⇓ inl result
   | state, logs }}.
 Proof.
@@ -775,14 +826,13 @@ Qed.
 
 Lemma transfer_from_to_is_valid
     (storage : erc20.Erc20.t)
-    (logs : M.Logs)
     (from : erc20.AccountId.t)
     (to : erc20.AccountId.t)
     (value : ltac:(erc20.Balance))
     (H_storage : Erc20.Valid.t storage)
     (H_value : Integer.Valid.t value) :
   let '(result, (storage, _)) :=
-    Simulations.erc20.transfer_from_to from to value (storage, logs) in
+    Simulations.erc20.transfer_from_to from to value (storage, []) in
   match result with
   | inl _ => Erc20.Valid.t storage
   | _ => True
@@ -833,7 +883,7 @@ Proof.
     pose proof H_storage.(Erc20.Valid.sum _) as H_sum_eq.
     unfold sum_of_money in H_sum_eq; cbn in H_sum_eq; rewrite <- H_sum_eq.
     clear H_sum_eq.
-    destruct (account_id_eq_neq to from) as [H_to_from_eq | H_to_from_neq].
+    destruct (AccountId.eq_or_neq to from) as [H_to_from_eq | H_to_from_neq].
     { rewrite H_to_from_eq in *; clear H_to_from_eq.
       unfold erc20.balance_of_impl in *; cbn.
       rewrite Lib.Mapping.get_insert_eq; cbn.
@@ -849,13 +899,12 @@ Qed.
 Lemma transfer_is_valid
     (env : erc20.Env.t)
     (storage : erc20.Erc20.t)
-    (logs : M.Logs)
     (to : erc20.AccountId.t)
     (value : ltac:(erc20.Balance))
     (H_storage : Erc20.Valid.t storage)
     (H_value : Integer.Valid.t value) :
-  let '(result, (storage, logs)) :=
-    Simulations.erc20.transfer env to value (storage, logs) in
+  let '(result, (storage, _)) :=
+    Simulations.erc20.transfer env to value (storage, []) in
   match result with
   | inl _ => Erc20.Valid.t storage
   | _ => True
@@ -867,13 +916,12 @@ Qed.
 Lemma approve_is_valid
     (env : erc20.Env.t)
     (storage : erc20.Erc20.t)
-    (logs : M.Logs)
     (spender : erc20.AccountId.t)
     (value : ltac:(erc20.Balance))
     (H_storage : Erc20.Valid.t storage)
     (H_value : Integer.Valid.t value) :
   let '(result, (storage, _)) :=
-    Simulations.erc20.approve env spender value (storage, logs) in
+    Simulations.erc20.approve env spender value (storage, []) in
   Erc20.Valid.t storage.
 Proof.
   cbn.
@@ -885,14 +933,13 @@ Qed.
 Lemma transfer_from_is_valid
     (env : erc20.Env.t)
     (storage : erc20.Erc20.t)
-    (logs : M.Logs)
     (from : erc20.AccountId.t)
     (to : erc20.AccountId.t)
     (value : ltac:(erc20.Balance))
     (H_storage : Erc20.Valid.t storage)
     (H_value : Integer.Valid.t value) :
   let '(result, (storage, _)) :=
-    Simulations.erc20.transfer_from env from to value (storage, logs) in
+    Simulations.erc20.transfer_from env from to value (storage, []) in
   match result with
   | inl _ => Erc20.Valid.t storage
   | _ => True
@@ -902,7 +949,7 @@ Proof.
   unfold BinOp.Pure.lt, BinOp.Pure.make_comparison; cbn.
   destruct (_ <? _) eqn:H_lt; [trivial|].
   pose proof (H_transfer :=
-    transfer_from_to_is_valid storage logs from to value H_storage H_value).
+    transfer_from_to_is_valid storage from to value H_storage H_value).
   unfold M.StateError.bind.
   destruct Simulations.erc20.transfer_from_to
     as [[?result|?exception] [?storage ?logs]];
@@ -921,13 +968,12 @@ Qed.
 Lemma write_dispatch_is_valid
     (env : erc20.Env.t)
     (storage : erc20.Erc20.t)
-    (logs : M.Logs)
     (write_message : WriteMessage.t)
     (H_storage : Erc20.Valid.t storage)
     (H_write_message : WriteMessage.Valid.t write_message) :
   let state := State.of_storage storage in
   let '(result, (storage, _)) :=
-    WriteMessage.simulation_dispatch env write_message (storage, logs) in
+    WriteMessage.simulation_dispatch env write_message (storage, []) in
   match result with
   | inl _ => Erc20.Valid.t storage
   | _ => True
@@ -943,12 +989,11 @@ Qed.
 Module Sum_of_money_is_constant.
   Lemma transfer_from_to_constant
       (storage : erc20.Erc20.t)
-      (logs : M.Logs)
       (from : erc20.AccountId.t)
       (to : erc20.AccountId.t)
       (value : ltac:(erc20.Balance)) :
     let '(result, (storage', _)) :=
-      Simulations.erc20.transfer_from_to from to value (storage, logs) in
+      Simulations.erc20.transfer_from_to from to value (storage, []) in
     match result with
     | inl _ =>
       storage.(erc20.Erc20.total_supply) =
@@ -963,11 +1008,10 @@ Module Sum_of_money_is_constant.
   Lemma transfer_is_constant
       (env : erc20.Env.t)
       (storage : erc20.Erc20.t)
-      (logs : M.Logs)
       (to : erc20.AccountId.t)
       (value : ltac:(erc20.Balance)) :
     let '(result, (storage', _)) :=
-      Simulations.erc20.transfer env to value (storage, logs) in
+      Simulations.erc20.transfer env to value (storage, []) in
     match result with
     | inl _ =>
       storage.(erc20.Erc20.total_supply) =
@@ -981,11 +1025,10 @@ Module Sum_of_money_is_constant.
   Lemma approve_is_constant
       (env : erc20.Env.t)
       (storage : erc20.Erc20.t)
-      (logs : M.Logs)
       (spender : erc20.AccountId.t)
       (value : ltac:(erc20.Balance)) :
     let '(result, (storage', _)) :=
-      Simulations.erc20.approve env spender value (storage, logs) in
+      Simulations.erc20.approve env spender value (storage, []) in
     match result with
     | inl _ =>
       storage.(erc20.Erc20.total_supply) =
@@ -999,12 +1042,11 @@ Module Sum_of_money_is_constant.
   Lemma transfer_from_is_constant
       (env : erc20.Env.t)
       (storage : erc20.Erc20.t)
-      (logs : M.Logs)
       (from : erc20.AccountId.t)
       (to : erc20.AccountId.t)
       (value : ltac:(erc20.Balance)) :
     let '(result, (storage', _)) :=
-      Simulations.erc20.transfer_from env from to value (storage, logs) in
+      Simulations.erc20.transfer_from env from to value (storage, []) in
     match result with
     | inl _ =>
       storage.(erc20.Erc20.total_supply) =
@@ -1014,7 +1056,7 @@ Module Sum_of_money_is_constant.
   Proof.
     cbn.
     step; cbn; trivial.
-    pose proof (transfer_from_to_constant storage logs from to value).
+    pose proof (transfer_from_to_constant storage from to value).
     unfold M.StateError.bind.
     destruct Simulations.erc20.transfer_from_to; cbn.
     repeat (step; cbn; trivial).
@@ -1023,11 +1065,10 @@ Module Sum_of_money_is_constant.
   Lemma write_dispatch_is_constant
       (env : erc20.Env.t)
       (storage : erc20.Erc20.t)
-      (logs : M.Logs)
       (write_message : WriteMessage.t) :
     let state := State.of_storage storage in
     let '(result, (storage', _)) :=
-      WriteMessage.simulation_dispatch env write_message (storage, logs) in
+      WriteMessage.simulation_dispatch env write_message (storage, []) in
     match result with
     | inl _ =>
       storage.(erc20.Erc20.total_supply) =
@@ -1041,3 +1082,188 @@ Module Sum_of_money_is_constant.
     { now apply transfer_from_is_constant. }
   Qed.
 End Sum_of_money_is_constant.
+
+(** ** We describe what action occured on the storage, according to the logs. *)
+Module Action_from_log.
+  Module Action.
+    (** An action on the storage is described by a proposition relating the
+        value of the storage before and after. We use a proposition rather than
+        a function as there can be many possible final storage given what we
+        know from the logs. *)
+    Definition t : Type := erc20.Erc20.t -> erc20.Erc20.t -> Prop.
+  End Action.
+
+  (** The new value of the field [balances] of the storage after a tranfer. Here
+      we ignore the overflow on integers as we consider the operation
+      successful. *)
+  Definition balances_of_transfer
+      (storage : erc20.Erc20.t)
+      (from to : erc20.AccountId.t)
+      (value : ltac:(erc20.Balance)) :
+      erc20.Mapping.t erc20.AccountId.t ltac:(erc20.Balance) :=
+    if AccountId.eqb from to then
+      (* Inserting its own value can be useful to initialize an account *)
+      Lib.Mapping.insert
+        from
+        (Simulations.erc20.balance_of_impl storage from)
+        storage.(erc20.Erc20.balances)
+    else
+      let from_value := Simulations.erc20.balance_of_impl storage from in
+      let to_value := Simulations.erc20.balance_of_impl storage to in
+      Lib.Mapping.insert from (BinOp.Optimistic.sub from_value value)
+      (Lib.Mapping.insert to (BinOp.Optimistic.add to_value value)
+      storage.(erc20.Erc20.balances)).
+
+  (** The action on the storage that we can infer from an event. *)
+  Definition action_of_event (event : erc20.Event.t) : Action.t :=
+    fun storage storage' =>
+    match event with
+    | erc20.Event.Transfer (erc20.Transfer.Build_t
+        (option.Option.Some from)
+        (option.Option.Some to)
+        value
+      ) =>
+      (* In case of transfer event, we do not know how the allowances are
+         updated. *)
+      exists allowances',
+      storage' =
+      storage <|
+        erc20.Erc20.balances := balances_of_transfer storage from to value
+      |> <|
+        erc20.Erc20.allowances := allowances'
+      |>
+    | erc20.Event.Transfer (erc20.Transfer.Build_t _ _ _) => False
+    | erc20.Event.Approval (erc20.Approval.Build_t owner spender value) =>
+      storage' =
+      storage <|
+        erc20.Erc20.allowances :=
+          Lib.Mapping.insert (owner, spender) value
+            storage.(erc20.Erc20.allowances)
+      |>
+    end.
+
+  (** Iterate the events. Actually, in this example, there is at most one event
+      per primitive of the smart contract
+      Note that we apply the events in the reverse order, as the last event is
+      added last in the list, and thus appear at the head. *)
+  Fixpoint action_of_events (events : list erc20.Event.t) : Action.t :=
+    fun storage storage' =>
+    match events with
+    | [] => storage' = storage
+    | event :: events =>
+      exists storage_inter,
+      action_of_event event storage_inter storage' /\
+      action_of_events events storage storage_inter
+    end.
+
+  (** The effect on the storage of the function [transfer_from_to]. *)
+  Lemma transfer_from_to_on_storage
+      (storage : erc20.Erc20.t)
+      (from to : erc20.AccountId.t)
+      (value : ltac:(erc20.Balance)) :
+    match
+      Simulations.erc20.transfer_from_to from to value (storage, [])
+    with
+    | (inl (result.Result.Ok tt), (storage', _)) =>
+      storage' =
+      storage <|
+        erc20.Erc20.balances := balances_of_transfer storage from to value
+      |>
+    | _ => True
+    end.
+  Proof.
+    cbn.
+    destruct (_ <u128 _) eqn:?; cbn; [easy|].
+    unfold
+      BinOp.Error.add,
+      BinOp.Error.make_arithmetic,
+      Integer.normalize_error.
+    do 2 (destruct (_ <? _); cbn; [easy|]).
+    unfold balances_of_transfer.
+    destruct AccountId.eqb eqn:?.
+    { replace to with from in * by (apply AccountId.eqb_true; assumption).
+      set (initial_value := Simulations.erc20.balance_of_impl _ _) in *.
+      unfold Simulations.erc20.balance_of_impl; cbn.
+      rewrite Lib.Mapping.get_insert_eq.
+      destruct storage; cbn.
+      unfold RecordUpdate.set; f_equal.
+      rewrite Lib.Mapping.insert_insert by apply AccountId.eq_or_neq.
+      f_equal.
+      destruct initial_value as [initial_value], value as [value].
+      f_equal.
+      lia.
+    }
+    { assert (from <> to) by now apply AccountId.eqb_false.
+      destruct storage; cbn.
+      unfold RecordUpdate.set; f_equal.
+      unfold Simulations.erc20.balance_of_impl in *; cbn in *.
+      rewrite Lib.Mapping.get_insert_neq by congruence.
+      set (from_value := Lib.Mapping.get from _) in *.
+      set (to_value := Lib.Mapping.get to _) in *.
+      destruct
+        from_value as [|[from_value]],
+        to_value as [|[to_value]],
+        value as [value].
+      all: rewrite Lib.Mapping.insert_switch;
+        try apply AccountId.eq_or_neq;
+        try congruence.
+    }
+  Qed.
+
+  (** The logs of the function [transfer_from_to]. *)
+  Lemma event_from_transfer_from_to
+      (storage : erc20.Erc20.t)
+      (from to : erc20.AccountId.t)
+      (value : ltac:(erc20.Balance)) :
+    match
+      Simulations.erc20.transfer_from_to from to value (storage, [])
+    with
+    | (inl (result.Result.Ok tt), (_, events)) =>
+      let event := erc20.Event.Transfer {|
+        erc20.Transfer.from := option.Option.Some from;
+        erc20.Transfer.to := option.Option.Some to;
+        erc20.Transfer.value := value;
+      |} in
+      [event] = events
+    | _ => True
+    end.
+  Proof.
+    cbn.
+    destruct (_ <u128 _); cbn; [easy|].
+    now destruct BinOp.Error.add.
+  Qed.
+
+  (** We show that the action that we infer from the logs is indeed what is
+      happening on the storage. *)
+  Lemma retrieve_action_from_logs
+      (env : erc20.Env.t)
+      (storage : erc20.Erc20.t)
+      (write_message : WriteMessage.t)
+      (events : list erc20.Event.t) :
+    match
+      WriteMessage.simulation_dispatch env write_message (storage, [])
+    with
+    | (inl (result.Result.Ok tt), (storage', events)) =>
+      action_of_events events storage storage'
+    | _ => True
+    end.
+  Proof.
+    Opaque Simulations.erc20.transfer_from_to.
+    destruct write_message; cbn;
+      unfold Simulations.erc20.transfer, M.StateError.bind;
+      try (destruct (_ <u128 _) eqn:?; cbn; [easy|]);
+      try match goal with
+      | |- context[erc20.transfer_from_to ?from ?to ?value (?storage, [])] =>
+        pose proof (
+          transfer_from_to_on_storage storage from to value
+        );
+        pose proof (
+          event_from_transfer_from_to storage from to value
+        )
+      end;
+      try destruct Simulations.erc20.transfer_from_to
+        as [[[[]|?error]|?exception] [?storage ?events]];
+      hauto l: on.
+    Transparent Simulations.erc20.transfer_from_to.
+  Qed.
+End Action_from_log.
