CoqOfRust/examples/default/examples/ink_contracts/Simulations/erc20.v
@@ -10,8 +10,11 @@ Module Env.
   Definition caller (self : erc20.Env.t) : erc20.AccountId.t :=
     self.(erc20.Env.caller).
 
-  Definition emit_event : unit :=
-    tt.
+  Definition emit_event
+      (events : list erc20.Event.t)
+      (event : erc20.Event.t) :
+      list erc20.Event.t :=
+    event :: events.
 End Env.
 
 Definition env (env : erc20.Env.t) : erc20.Env.t :=
@@ -56,12 +59,16 @@ Definition allowance
 
 (** ** Simulations modifying the state. *)
 
+Module State.
+  Definition t : Set := erc20.Erc20.t * list erc20.Event.t.
+End State.
+
 Definition transfer_from_to
     (from : erc20.AccountId.t)
     (to : erc20.AccountId.t)
     (value : ltac:(erc20.Balance)) :
-    MS? (erc20.Erc20.t * M.Logs) ltac:(erc20.Result unit) :=
-  letS? '(storage, logs) := readS? in
+    MS? State.t ltac:(erc20.Result unit) :=
+  letS? '(storage, events) := readS? in
   let from_balance := balance_of_impl storage from in
   if from_balance <u128 value then
     returnS? (result.Result.Err erc20.Error.InsufficientBalance)
@@ -72,12 +79,12 @@ Definition transfer_from_to
         Lib.Mapping.insert from new_from_balance
           storage.(erc20.Erc20.balances)
       |>,
-      logs
+      events
     ) in
-    letS? '(storage, logs) := readS? in
+    letS? '(storage, events) := readS? in
     let to_balance := balance_of_impl storage to in
     letS? new_to_balance := return?toS? (BinOp.Error.add to_balance value) in
-    let event := {|
+    let event := erc20.Event.Transfer {|
       erc20.Transfer.from := option.Option.Some from;
       erc20.Transfer.to := option.Option.Some to;
       erc20.Transfer.value := value
@@ -87,7 +94,7 @@ Definition transfer_from_to
         Lib.Mapping.insert to new_to_balance
           storage.(erc20.Erc20.balances)
       |>,
-      existS _ event :: logs
+      event :: events
     ) in
     returnS? (result.Result.Ok tt).
 
@@ -95,17 +102,17 @@ Definition transfer
     (env : erc20.Env.t)
     (to : erc20.AccountId.t)
     (value : ltac:(erc20.Balance)) :
-    MS? (erc20.Erc20.t * M.Logs) ltac:(erc20.Result unit) :=
+    MS? State.t ltac:(erc20.Result unit) :=
   transfer_from_to (Env.caller env) to value.
 
 Definition approve
     (env : erc20.Env.t)
     (spender : erc20.AccountId.t)
     (value : ltac:(erc20.Balance)) :
-    MS? (erc20.Erc20.t * M.Logs) ltac:(erc20.Result unit) :=
+    MS? State.t ltac:(erc20.Result unit) :=
   let owner := Env.caller env in
-  letS? '(storage, logs) := readS? in
-  let event := {|
+  letS? '(storage, events) := readS? in
+  let event := erc20.Event.Approval {|
     erc20.Approval.owner := (erc20.env env).(ink_contracts.erc20.Env.caller);
     erc20.Approval.spender := spender;
     erc20.Approval.value := value
@@ -115,7 +122,7 @@ Definition approve
       Lib.Mapping.insert (owner, spender) value
         storage.(erc20.Erc20.allowances)
     |>,
-    existS _ event :: logs
+    event :: events
   ) in
   returnS? (result.Result.Ok tt).
 
@@ -124,9 +131,9 @@ Definition transfer_from
     (from : erc20.AccountId.t)
     (to : erc20.AccountId.t)
     (value : ltac:(erc20.Balance)) :
-    MS? (erc20.Erc20.t * M.Logs) ltac:(erc20.Result unit) :=
+    MS? State.t ltac:(erc20.Result unit) :=
   let caller := Env.caller env in
-  letS? '(storage, logs) := readS? in
+  letS? '(storage, events) := readS? in
   let allowance := allowance_impl storage from caller in
   if allowance <u128 value then
     returnS? (result.Result.Err erc20.Error.InsufficientAllowance)
@@ -136,13 +143,13 @@ Definition transfer_from
     | result.Result.Err _ => returnS? (result_from_to)
     | result.Result.Ok _ =>
       let new_allowance := BinOp.Optimistic.sub allowance value in
-      letS? '(storage, logs) := readS? in
+      letS? '(storage, events) := readS? in
       letS? _ := writeS? (
         storage <| erc20.Erc20.allowances :=
           Lib.Mapping.insert (from, caller) new_allowance
             storage.(erc20.Erc20.allowances)
         |>,
-        logs
+        events
       ) in
       returnS? (result.Result.Ok tt)
     end.
