CoqOfRust/examples/default/examples/ink_contracts/Proofs/Lib.v
@@ -4,8 +4,6 @@ Require Import CoqOfRust.examples.default.examples.ink_contracts.Lib.
 
 Module  Mapping.
 Section Mapping.
-  Parameter t : Set -> Set -> Set.
-
   Context {K V : Set}.
   Context (K_eq_neq : forall (k1 k2 : K), k1 = k2 \/ k1 <> k2).
 
@@ -21,6 +19,60 @@ Section Mapping.
   Axiom get_insert_neq : forall (k1 k2 : K) (v : V) m,
     k1 <> k2 ->
     Mapping.get k1 (Mapping.insert k2 v m) = Mapping.get k1 m.
+
+  (** ** [get/equality] rule *)
+
+  Axiom get_all_equal : forall (m1 m2 : Lib.Mapping.t K V),
+    (forall k, Mapping.get k m1 = Mapping.get k m2) ->
+    m1 = m2.
+
+  Lemma insert_insert (k : K) (v1 v2 : V) m :
+    Mapping.insert k v2 (Mapping.insert k v1 m) = Mapping.insert k v2 m.
+  Proof.
+    apply get_all_equal; intros k'.
+    destruct (K_eq_neq k k') as [H_eq | H_neq].
+    { rewrite H_eq.
+      now repeat rewrite get_insert_eq.
+    }
+    { repeat rewrite get_insert_neq; congruence. }
+  Qed.
+
+  Lemma insert_id (k : K) (v : V) m :
+    Mapping.get k m = option.Option.Some v ->
+    Mapping.insert k v m = m.
+  Proof.
+    intros H_get.
+    apply get_all_equal; intros k'.
+    destruct (K_eq_neq k k') as [H_eq | H_neq].
+    { rewrite H_eq.
+      rewrite get_insert_eq.
+      congruence.
+    }
+    { rewrite get_insert_neq; congruence. }
+  Qed.
+
+  Lemma insert_switch (k1 k2 : K) (v1 v2 : V) m :
+    k1 <> k2 ->
+    Mapping.insert k1 v1 (Mapping.insert k2 v2 m) =
+    Mapping.insert k2 v2 (Mapping.insert k1 v1 m).
+  Proof.
+    intros H_neq.
+    apply get_all_equal; intros k'.
+    destruct (K_eq_neq k1 k') as [H_eq1 | H_neq1];
+      destruct (K_eq_neq k2 k') as [H_eq2 | H_neq2].
+    { congruence. }
+    { subst.
+      rewrite get_insert_eq.
+      rewrite get_insert_neq by congruence.
+      now rewrite get_insert_eq.
+    }
+    { subst.
+      rewrite get_insert_eq.
+      rewrite get_insert_neq by congruence.
+      now rewrite get_insert_eq.
+    }
+    { repeat rewrite get_insert_neq; congruence. }
+  Qed.
 
   (** ** [sum] rules *)
 
